{-# OPTIONS --safe --without-K #-}

module Lambda where

open import Type public
open import Context Ty public

open import Presheaf.Base ğ’² public
open import Presheaf.CartesianClosure ğ’² public

open import Data.Product using (Î£; _Ã—_; _,_ ; projâ‚ ; projâ‚‚)

open import Relation.Binary.PropositionalEquality
  using    (_â‰¡_ ; refl ; cong ; congâ‚‚ ; module â‰¡-Reasoning ; subst ; substâ‚‚)
  renaming (sym to â‰¡-sym ; trans to â‰¡-trans ; isEquivalence to â‰¡-equiv)

-- Variable presheaf
Var' : Ty â†’ Psh
Var' Ï„ = record
          { Fam           = Î» Î“ â†’ Var Î“ Ï„
          ; _â‰‹_           = _â‰¡_
          ; â‰‹-equiv       = Î» _ â†’ â‰¡-equiv
          ; wk            = wkVar
          ; wk-pres-â‰‹     = Î» w xâ‰‹y â†’ cong (wkVar w) xâ‰‹y
          ; wk-pres-refl  = wkVar-pres-refl
          ; wk-pres-trans = wkVar-pres-trans
          }

-- Extension functor
Îµ[_]_ : Ty â†’ Psh â†’ Psh
Îµ[ Ï„ ] ğ’« = record
       { Fam           = Î» Î“ â†’ ğ’« â‚€ (Î“ `, Ï„)
       ; _â‰‹_           = Î» x y â†’ x â‰‹[ ğ’« ] y
       ; â‰‹-equiv       = Î» Î“ â†’ Psh.â‰‹-equiv ğ’« (Î“ `, Ï„)
       ; wk            = Î» r â†’ wk[ ğ’« ] (âŠ†-keep r)
       ; wk-pres-â‰‹     = Î» r â†’ wk[ ğ’« ]-pres-â‰‹ (âŠ†-keep r)
       ; wk-pres-refl  = Î» x â†’ wk[ ğ’« ]-pres-refl x
       ; wk-pres-trans = Î» w w' x â†’ â‰‹[ ğ’« ]-trans
         (â‰‹[ ğ’« ]-reflexive (cong (Î» r â†’ wk[ ğ’« ] r x) (âŠ†-keep-pres-trans w w')))
         (wk[ ğ’« ]-pres-trans (âŠ†-keep w) (âŠ†-keep w') x)
       }

Îµ[_]-map : {ğ’« ğ’¬ : Psh} (Ï„ : Ty) â†’ (ğ’« â†’Ì‡ ğ’¬) â†’ Îµ[ Ï„ ] ğ’« â†’Ì‡ Îµ[ Ï„ ] ğ’¬
Îµ[_]-map Ï„ f = record
  { fun     = f .apply
  ; pres-â‰‹  = f .apply-â‰‹
  ; natural = Î» w p â†’ f .natural (âŠ†-keep w) p
  }

record LambdaAlgebra (ğ’¯ : Ty â†’ Psh) : Setâ‚ where
  field
    var : Var' Ï„ â†’Ì‡ ğ’¯ Ï„
    lam : Îµ[ Ïƒ ] (ğ’¯ Ï„) â†’Ì‡ ğ’¯ (Ïƒ â‡’ Ï„)
    app : ğ’¯ (Ïƒ â‡’ Ï„) Ã—' ğ’¯ Ïƒ â†’Ì‡ ğ’¯ Ï„

  Tm : Ctx â†’ Ty â†’ Set
  Tm Î“ Ï„ = ğ’¯ Ï„ â‚€ Î“

  _â‰ˆ_ : {Ï„ : Ty} â†’ (t t' : Tm Î“ Ï„) â†’ Set
  t â‰ˆ t' = t â‰‹[ ğ’¯ _ ] t'

  â‰ˆ-refl : {t : Tm Î“ Ï„} â†’ t â‰ˆ t
  â‰ˆ-refl = â‰‹[ ğ’¯ _ ]-refl

  â‰ˆ-sym : {t t' : Tm Î“ Ï„} â†’ t â‰ˆ t' â†’ t' â‰ˆ t
  â‰ˆ-sym = â‰‹[ ğ’¯ _ ]-sym

  â‰ˆ-trans : {t t' t'' : Tm Î“ Ï„} â†’ t â‰ˆ t' â†’ t' â‰ˆ t'' â†’ t â‰ˆ t''
  â‰ˆ-trans = â‰‹[ ğ’¯ _ ]-trans
  
